mlApplyMetaGeneralized (#306)
* comments

restructure some lemmas

simplify some lemmas

* decide_eq_same

* simplify/refactor a lemma

* use decide_eq_same

* lhs_imp_to_and

* Reshaper: lhs_imp_to_and_r

* more resharper

* WIP generalizing mlApply[Meta]

* WIP debugging

* 'mlApplyMetaGeneralized' works, but ...

... generates wrong order of assumptions

* xs ++ [x]

* To be reverted

* Revert "To be reverted"

This reverts commit 67a52fbc483f9754d7a75e534d697c9b36c48c20.

* Revert "xs ++ [x]"

This reverts commit c2c2f1c0db832af778873aa01e3d2e398ee5f14d.

* WIP

* foldr_and_weaken_last

* foldr_and_last_rotate

* foldr_and_last_rotate_(1|2)

* WIP

* [reshape_lhs_imp_to_and_forward'], [reshape_lhs_imp_to_and_forward]

* ex_mlApplyMetaGeneralized

* minor fix

matching-logic/src/ProofMode_reshaper.v
@@ -2,7 +2,7 @@ From Coq Require Import ssreflect ssrfun ssrbool.
 
 From Ltac2 Require Import Ltac2.
 
-From Coq Require Import Ensembles Bool.
+From Coq Require Import Ensembles Bool String.
 From Coq.Logic Require Import FunctionalExtensionality Eqdep_dec.
 From Equations Require Import Equations.
 
@@ -14,6 +14,7 @@ From MatchingLogic Require Import
     ProofSystem
     IndexManipulation
     wftactics
+    ProofInfo
     ProofMode_base
     ProofMode_propositional
 .
@@ -31,6 +32,10 @@ Import
 .
 
 Set Default Proof Mode "Classic".
+
+Open Scope ml_scope.
+Open Scope string_scope.
+Open Scope list_scope.
 
 Section with_signature.
   Context {Σ : Signature}.
@@ -134,7 +139,12 @@ Section with_signature.
   Abort.
 
 
-  Lemma lhs_and_to_imp_r Γ (g x : Pattern) (xs : list Pattern) i :
+  (*
+    Γ ⊢ (φ₁ and ... and φₖ) ---> ψ
+    -------------------------------
+    Γ ⊢ φ₁ ---> ... ---> φₖ ---> ψ
+  *)
+  Lemma reshape_lhs_imp_to_and_backward Γ (g x : Pattern) (xs : list Pattern) i :
     well_formed g ->
     well_formed x ->
     Pattern.wf xs ->
@@ -149,16 +159,279 @@ Section with_signature.
     apply lhs_and_to_imp_meta; assumption.
   Defined.
 
+  Lemma reshape_lhs_imp_to_and_forward' Γ (g x : Pattern) (xs : list Pattern) i :
+    well_formed g ->
+    well_formed x ->
+    Pattern.wf xs ->
+    forall (r : ImpReshapeS g (x::xs)),
+       Γ ⊢i untagPattern (irs_flattened _ _ r) using i ->
+       Γ ⊢i ((foldr (patt_and) x xs) ---> g) using i.
+  Proof.
+    intros wfg wfx wfxs r H.
+    eapply cast_proof' in H.
+    2: { rewrite irs_pf; reflexivity. }
+    clear r.
+    apply lhs_imp_to_and_meta; assumption.
+  Defined.
 
-  Local Example ex_match Γ a b c d:
+  (*
+      Γ ⊢ φ₁ ---> ... ---> φₖ ---> ψ
+      ------------------------------
+      Γ ⊢ (φ₁ and ... and φₖ) ---> ψ
+  *)
+  Lemma reshape_lhs_imp_to_and_forward Γ (g x : Pattern) (xs : list Pattern) i :
+    well_formed g ->
+    well_formed x ->
+    Pattern.wf xs ->
+    forall (r : ImpReshapeS g (x::xs)),
+       Γ ⊢i untagPattern (irs_flattened _ _ r) using i ->
+       match (rev xs) with
+       | [] => Γ ⊢i x ---> g using i
+       | yk::ys =>
+          Γ ⊢i ((foldr (patt_and) yk (x::(rev ys))) ---> g) using i
+       end.
+  Proof.
+    intros wfg wfx wfxs r H.
+    apply reshape_lhs_imp_to_and_forward' in H;[|assumption|assumption|assumption].
+    destruct (rev xs) eqn:Heqxs; simpl in *.
+    {
+      apply (f_equal (@rev Pattern)) in Heqxs.
+      rewrite rev_involutive in Heqxs.
+      simpl in Heqxs.
+      subst xs. simpl in H.
+      exact H.
+    }
+    {
+      rewrite -[xs]rev_involutive in H.
+      rewrite Heqxs in H.
+      simpl in H.
+      destruct xs as [|y ys];[(simpl in Heqxs; inversion Heqxs)|].
+      simpl in Heqxs.
+
+      apply (f_equal (@rev Pattern)) in Heqxs.
+      simpl in Heqxs.
+      rewrite rev_app_distr in Heqxs.
+      simpl in Heqxs.
+      rewrite rev_involutive in Heqxs.
+
+      assert (Pattern.wf l).
+      {
+        rewrite Heqxs in wfxs.
+        apply wfapp_proj_1 in wfxs.
+        rewrite -[l]rev_involutive.
+        apply wf_rev.
+        apply wfxs.
+      }
+
+      assert (well_formed p).
+      {
+        rewrite Heqxs in wfxs.
+        apply wfapp_proj_2 in wfxs.
+        unfold Pattern.wf in wfxs. simpl in wfxs.
+        destruct_and!; assumption.
+      }
+
+      assert (Pattern.wf (rev l)).
+      { apply wf_rev. assumption. }
+
+      assert (well_formed (foldr patt_and x l)).
+      { apply well_formed_foldr_and; assumption. }
+
+      assert (well_formed (foldr patt_and p l)).
+      { apply well_formed_foldr_and; assumption. }
+
+      assert (well_formed (foldr patt_and (p and x) l)).
+      { apply well_formed_foldr_and; wf_auto2. }
+
+
+      assert (well_formed (foldr patt_and x (rev l))).
+      { apply well_formed_foldr_and; assumption. }
+
+      assert (well_formed (foldr patt_and p (rev l))).
+      { apply well_formed_foldr_and; assumption. }
+
+      assert (well_formed (foldr patt_and (p and x) (rev l))).
+      { apply well_formed_foldr_and; wf_auto2. }
+
+      toMLGoal.
+      {
+        apply well_formed_imp;[|assumption].
+        apply well_formed_and;[assumption|].
+        apply well_formed_foldr_and; assumption.
+      }
+      
+      mlAdd H as "H1".
+      mlIntro "H2".
+      mlApply "H1".
+      mlClear "H1".
+      rewrite foldr_app.
+      simpl.
+      useBasicReasoning.
+      mlAdd (foldr_and_weaken_last Γ p (p and x) (rev l) ltac:(wf_auto2) ltac:(wf_auto2) ltac:(wf_auto2)) as "Hw".
+      mlDestructAnd "H2" as "Hx" "Hf".
+      mlAssert ("Hw'": (foldr patt_and p (rev l) ---> foldr patt_and (p and x) (rev l))).
+      { wf_auto2. }
+      {
+        mlApply "Hw".
+        mlIntro "Hp".
+        mlSplitAnd;[mlExact "Hp" | mlExact "Hx"].
+      }
+      mlClear "Hw".
+      mlApply "Hw'".
+      mlExact "Hf".
+    }
+  Defined.
+
+  Local Example ex_match_imp Γ a b c d:
     well_formed a ->
     well_formed b ->
     well_formed c ->
     well_formed d ->
+    Γ ⊢i c ---> (b ---> (a ---> d)) using BasicReasoning ->
     Γ ⊢i a ---> (b ---> (c ---> d)) using BasicReasoning.
   Proof.
+    intros wfa wfb wfc wfd H.
+    apply reshape_lhs_imp_to_and_backward; try_wfauto2.
+    apply reshape_lhs_imp_to_and_forward in H; try_wfauto2.
+    simpl in *.
+  Abort.
+
+
+  Structure AndReshapeS (g : Pattern) (l : list Pattern) :=
+  AndReshape
+    { ars_flattened :> TaggedPattern ;
+      ars_pf : (untagPattern ars_flattened) = foldr patt_and g l ;
+    }.
+
+  Lemma AndReshape_nil_pf0:
+    ∀ (g : Pattern),
+      g = foldr patt_and g [].
+  Proof. intros. reflexivity. Qed.
+
+  Canonical Structure AndReshape_nil (g : Pattern) : AndReshapeS g [] :=
+    AndReshape g [] (reshape_nil g) (AndReshape_nil_pf0 g).
+
+
+  Program Canonical Structure AndReshape_cons
+     (g x : Pattern) (xs : list Pattern) (r : AndReshapeS g xs)
+  : AndReshapeS g (x::xs) :=
+    AndReshape g (x::xs) (reshape_cons (x and untagPattern (reshape_cons r))) _.
+  Next Obligation.
+    intros g x xs r. simpl.
+    rewrite ars_pf.
+    reflexivity.
+  Qed.
+
+
+  Lemma reshape_and (Γ : Theory) (g : Pattern) (xs: list Pattern) (i : ProofInfo) :
+    forall (r : AndReshapeS g xs),
+       Γ ⊢i foldr (patt_and) g xs using i ->
+       Γ ⊢i (untagPattern (ars_flattened _ _ r)) using i.
+  Proof.
+    intros r [pf Hpf].
+    unshelve (eexists).
+    {
+      eapply cast_proof.
+      { rewrite ars_pf; reflexivity. }
+      exact pf.
+    }
+    {
+      simpl.
+      destruct Hpf as [Hpf2 Hpf3 Hpf4].
+      constructor.
+      {
+        rewrite elem_of_subseteq in Hpf2.
+        rewrite elem_of_subseteq.
+        intros x Hx.
+        specialize (Hpf2 x).
+        apply Hpf2. clear Hpf2.
+        rewrite elem_of_gset_to_coGset in Hx.
+        rewrite uses_of_ex_gen_correct in Hx.
+        rewrite elem_of_gset_to_coGset.
+        rewrite uses_of_ex_gen_correct.
+        rewrite indifferent_to_cast_uses_ex_gen in Hx.
+        exact Hx.
+      }
+      {
+        rewrite elem_of_subseteq in Hpf3.
+        rewrite elem_of_subseteq.
+        intros x Hx.
+        specialize (Hpf3 x).
+        apply Hpf3. clear Hpf3.
+        rewrite elem_of_gset_to_coGset in Hx.
+        rewrite uses_of_svar_subst_correct in Hx.
+        rewrite elem_of_gset_to_coGset.
+        rewrite uses_of_svar_subst_correct.
+        rewrite indifferent_to_cast_uses_svar_subst in Hx.
+        exact Hx.
+      }
+      {
+        rewrite indifferent_to_cast_uses_kt.
+        apply Hpf4.
+      }
+      {
+        rewrite framing_patterns_cast_proof.
+        destruct i;assumption.
+      }
+    }
+  Defined.
+
+  Local Example ex_reshape_and Γ a b c d:
+  well_formed a ->
+  well_formed b ->
+  well_formed c ->
+  well_formed d ->
+  Γ ⊢i a and b and c and d using BasicReasoning.
+  Proof.
     intros wfa wfb wfc wfd.
-    apply lhs_and_to_imp_r.
+    apply reshape_and.
+  (* Now the goal has the right shape *)
+  Abort.
+
+    (*
+      Γ ⊢ φ₁ ---> ... ---> φₖ ---> ψ
+      ------------------------------
+      Γ ⊢ (φ₁ and ... and φₖ) ---> ψ
+    *)
+  Lemma reshape_lhs_and_to_imp_backward Γ (g x : Pattern) (xs : list Pattern) i :
+    well_formed g ->
+    well_formed x ->
+    Pattern.wf xs ->
+    forall (r : AndReshapeS x xs),
+       Γ ⊢i ((foldr (patt_imp) g (x::xs))) using i ->
+       Γ ⊢i (untagPattern (ars_flattened _ _ r)) ---> g using i .
+  Proof.
+    intros wfg wfx wfxs r H.
+    eapply cast_proof'.
+    { rewrite ars_pf; reflexivity. }
+    clear r.
+    apply lhs_imp_to_and_meta; assumption.
+  Defined.
+
+  Lemma reshape_lhs_and_to_imp_forward Γ (g x : Pattern) (xs : list Pattern) i :
+    well_formed g ->
+    well_formed x ->
+    Pattern.wf xs ->
+    forall (r : AndReshapeS x xs),
+      Γ ⊢i (untagPattern (ars_flattened _ _ r)) ---> g using i ->
+      Γ ⊢i ((foldr (patt_imp) g (x::xs))) using i.
+  Proof.
+    intros wfg wfx wfxs r H.
+    eapply cast_proof' in H.
+    2: { rewrite ars_pf; reflexivity. }
+    clear r.
+    apply lhs_and_to_imp_meta; assumption.
+  Defined.
+
+  Local Example ex_match_and Γ a b c d:
+   well_formed a ->
+   well_formed b ->
+   well_formed c ->
+   well_formed d ->
+   Γ ⊢i (a and b and c) ---> d using BasicReasoning.
+  Proof.
+   intros wfa wfb wfc wfd.
+   apply reshape_lhs_and_to_imp_backward; simpl.
   Abort.
 
 End with_signature.
